Based on the triangle rule of addition and subtraction with vectors, we can define
a triangle with sides a, b, a-b and θ is the angle between a and b.

Recall that the magnitude of a vector equals the squareroot of its dot product
so based on this we can state

||(a- b)|| = sqrt((a - b) ⋅ (a - b))
||(a- b)||^2 = (a - b) ⋅ (a - b)
Note that dot product distributes over vector addition and subtraction, which yields
||(a- b)||^2 = a ⋅ a - a ⋅ b - a ⋅ b + b ⋅ b
||(a- b)||^2 = (a ⋅ a) + (b ⋅ b) - 2(a ⋅ b)
Note that v ⋅ v = ||v||^2 which yields
||(a- b)||^2 = ||a||^2 + ||b||^2 - 2(a ⋅ b)
Note that a ⋅ b is equal to
||(a- b)||^2 = ||a||^2 + ||b||^2 - 2||a||||b||cosθ
