a. (sin(θ)/csc(θ)) + (cos(θ)/sec(θ)) = 1
(sin(θ)/csc(θ)) + (cos(θ)/sec(θ)) = 1
sin(θ) x 1/(1/sin(θ)) + cos(θ) x 1/(1/cos(θ))
sin^2(θ) + cos^2(θ) = 1

b. (sec^^2(θ) - 1)/sec^2(θ) = sin^2(θ)
(sec^^2(θ) - 1)/sec^2(θ) = sin^2(θ)
sec^^2(θ)/sec^2(θ) - 1/sec^2(θ) = sin^2(θ)
1 - 1/sec^2(θ) = sin^2(θ)
1 - 1/(1/cos^2(θ)) = sin^2(θ)
1 - cos^2(θ) = sin^2(θ)
1 = sin^2(θ) + cos^2(θ)

c. 1 + cot^2(θ) = csc^2(θ)
1 + cot^2(θ) = csc^2(θ)
1 + (cos^2(θ) / sin^2(θ)) = csc^2(θ)
(sin^2(θ)/ sin^2(θ)) + (cos^2(θ) / sin^2(θ)) = csc^2(θ)
(sin^2(θ) + cos^2(θ)) / sin^2(θ) = csc^2(θ)
1 / sin^2(θ) = csc^2(θ)

d. cos(θ)(tan(θ) + cot(θ)) = csc(θ)
cos(θ)(tan(θ) + cot(θ)) = csc(θ)
sin(θ) + cos^2(θ) / sin(θ) = csc(θ)
(sin^2(θ) + cos^2(θ)) / sin(θ) = csc(θ)
1 / sin(θ) = csc(θ)
